src/Pipit.Check.Example.Top.fst
@@ -1,0 +1,45 @@
+(* Top-level example *)
+module Pipit.Check.Example.Top
+
+open Pipit.Exp.Base
+
+open Pipit.System.Base
+open Pipit.System.Ind
+open Pipit.System.Exp
+
+module T = FStar.Tactics
+module Sugar = Pipit.Sugar
+
+let tac_nbe (): T.Tac unit = T.norm [primops; iota; delta; zeta; nbe]
+
+(*
+   count_when p =
+     let rec count =
+       (0 -> pre count) +
+       (if p then 1 else 0)
+*)
+inline_for_extraction
+let count_when (p: exp) =
+ let open Sugar in
+ mu' (
+   let count = XVar 0 in
+   let p' = lift' p in
+
+   (z0 --> pre count) +^ (ite p' z1 z0))
+
+(* forall e. count_when false <= count_when e <= count_when true *)
+let count_when_prop =
+  let open Sugar in
+  system_of_exp (
+    let' (count_when ff) (
+      let' (count_when x0) (
+        let' (count_when tt) (
+          let count_when_false = x2 in
+          let count_when_e = x1 in
+          let count_when_true = x0 in
+          count_when_false <=^ count_when_e /\ count_when_e <=^ count_when_true))))
+    1
+
+let count_when_prop_prove (): Lemma (ensures induct1' count_when_prop) =
+  assert (base_case' count_when_prop) by tac_nbe ();
+  assert (step_case' count_when_prop) by tac_nbe ()
