src/Pipit.Exec.Example.Manual.fst
@@ -1,0 +1,30 @@
+(* Manual translation example *)
+module Pipit.Exec.Example.Manual
+
+open LowStar.BufferOps
+
+module B = LowStar.Buffer
+module HS = FStar.HyperStack
+module G = FStar.Ghost
+module L = FStar.List.Tot
+module U32 = FStar.UInt32
+module MO = LowStar.Modifies
+
+open FStar.HyperStack.ST
+
+let init (state: B.pointer int): ST unit
+    (requires (fun h -> B.live h state))
+    (ensures (fun h _ h' -> B.live h' state)) =
+  state *= 0
+
+let eval (state: B.pointer int) (input: bool): ST int
+    (requires (fun h -> B.live h state))
+    (ensures (fun h _ h' -> B.live h' state)) =
+  let c = !* state in
+  c + (if input then 1 else 0)
+
+let update (state: B.pointer int) (input: bool): ST unit
+    (requires (fun h -> B.live h state))
+    (ensures (fun h _ h' -> B.live h' state)) =
+  let count' = eval state input in
+  state *= count'
