src/Pipit.Exec.LowStar.fst
@@ -1,0 +1,39 @@
+(* Shitty C translation *)
+module Pipit.Exec.LowStar
+
+// open Pipit.Exp.Base
+
+module X = Pipit.Exec.Base
+
+open LowStar.BufferOps
+
+module B = LowStar.Buffer
+module HS = FStar.HyperStack
+module G = FStar.Ghost
+module L = FStar.List.Tot
+module U32 = FStar.UInt32
+module MO = LowStar.Modifies
+
+open FStar.HyperStack.ST
+
+inline_for_extraction
+let mk_reset (#input #state #result: Type) (t: X.exec input state result) (stref: B.pointer state): ST unit
+    (requires (fun h -> B.live h stref))
+    (ensures (fun h _ h' -> B.live h' stref)) =
+  stref *= t.init
+
+inline_for_extraction
+let mk_step (#input #state #result: Type) (t: X.exec input state result) (inp: input) (stref: B.pointer state) : ST result
+    (requires (fun h -> B.live h stref))
+    (ensures (fun h _ h' -> B.live h' stref)) =
+  let st  = !*stref in
+  let res = t.eval inp st in
+  let st' = t.update inp st in
+  stref *= st';
+  res
+
+module Tac = FStar.Tactics
+
+let tac_post () =
+  Tac.norm [nbe; delta; primops; iota; zeta; delta_fully ["Pipit.System.ExpX.values_index"]];
+  Tac.trefl ()
