src/Pipit.Exp.ReactiveStep.fst
@@ -1,0 +1,63 @@
+module Pipit.Exp.ReactiveStep
+
+open Pipit.Exp.Base
+open Pipit.Exp.Subst
+
+module C = Pipit.Context
+
+let xBOTTOM = 0
+
+(* Reactive semantics:
+    react store e v e'
+   Under given heap, expression e produces value v and steps to e'
+ *)
+noeq type react (#inner: nat) (store: C.row inner): exp -> value -> exp -> Type =
+ | RVal: v: value ->
+         react store (XVal v) v (XVal v)
+
+ | RVar: x: var { x < inner } ->
+         react store (XVar x) (C.row_index store x) (XVar x)
+
+ | RPrim2: p: prim2 ->
+        e1:  exp   -> e2:  exp   ->
+        v1:  value -> v2:  value ->
+        e1': exp   -> e2': exp   ->
+        react store e1 v1 e1' ->
+        react store e2 v2 e2' ->
+        react store (XPrim2 p e1 e2) (eval_prim2 p v1 v2) (XPrim2 p e1' e2')
+
+ | RIte:
+        ep:  exp   -> e1:  exp   -> e2:  exp   ->
+        vp:  value -> v1:  value -> v2:  value ->
+        ep': exp   -> e1': exp   -> e2': exp   ->
+        react store ep vp ep' ->
+        react store e1 v1 e1' ->
+        react store e2 v2 e2' ->
+        react store (XIte ep e1 e2) (if vp <> 0 then v1 else v2) (XIte ep e1' e2')
+
+ | RPre: e1: exp -> v1: value -> e1': exp ->
+         react store e1 v1 e1' ->
+         react store (XPre e1) xBOTTOM (XThen (XVal v1) (XPre e1))
+
+ | RThen:
+        e1:  exp   -> e2:  exp   ->
+        v1:  value -> v2:  value ->
+        e1': exp   -> e2': exp   ->
+        react store e1 v1 e1' ->
+        react store e2 v2 e2' ->
+        react store (XThen e1 e2) v1 e2'
+
+ | RLet:
+        e1:  exp   -> e2:  exp   ->
+        v1:  value -> v2:  value ->
+        e1': exp   -> e2': exp   ->
+        react store e1 v1 e1' ->
+        react (C.row_append (C.row1 v1) store) e2 v2 e2' ->
+        react store (XLet e1 e2) v2 (XLet e1' e2')
+
+ | RMu:
+        e1:  exp   ->
+        v1:  value ->
+        e1': exp   ->
+        react (C.row_append (C.row1 v1) store) e1 v1 e1' ->
+        react store (XMu e1) v1 (XMu e1')
